meta/Criteria.fst
@@ -1,0 +1,311 @@
+module Criteria
+module STLC = STLC
+
+(** Relation between First Order Values of F* and STLC **)
+let rec (∽) (#t:STLC.fo_typ) (fs_v:STLC.elab_typ t) (#e:STLC.exp{STLC.is_value e}) (stlc_ht:STLC.typing STLC.empty e t) : Type0 =
+  match stlc_ht with
+  | STLC.TyUnit -> fs_v == ()
+  | STLC.TyZero -> fs_v == 0
+  | STLC.TySucc ht -> fs_v > 0 /\ (fs_v-1) ∽ ht
+  
+  | STLC.TyInl #_ #_ #t1 t2 ht1 ->
+    let fst_inl : either (STLC.elab_typ t1) (STLC.elab_typ t2) = fs_v in
+    Inl? fst_inl /\ (Inl?.v fst_inl ∽ ht1)
+  | STLC.TyInr #_ #_ t1 #t2 ht2 ->
+    let fs_inr : either (STLC.elab_typ t1) (STLC.elab_typ t2) = fs_v in
+    Inr? fs_inr /\ (Inr?.v fs_inr ∽ ht2)
+  | STLC.TyPair #_ #_ #_ #t1 #t2 ht_fst ht_snd ->
+    let (fs_fst, fs_snd) : (STLC.elab_typ t1 * STLC.elab_typ t2) = fs_v in
+    (fs_fst ∽ ht_fst) /\ (fs_snd ∽ ht_snd)
+
+(** *** Intrinsic criteria, static quoting/unquoting  **)
+type propS (t:STLC.fo_typ) = STLC.elab_typ t
+type propT (t:STLC.fo_typ) = e:STLC.exp{STLC.is_value e} & STLC.typing STLC.empty e t (** first order STLC value **)
+
+// let (⊆) (s0 s1:set_prop) : Type0 = False
+let (≌) (#t:STLC.fo_typ) (ss:propS t) (st:propT t) : Type0 =
+  ss ∽ (dsnd st)
+
+noeq type intS = { 
+  ct_stlc : STLC.typ;
+  // p_post : set_prop
+}
+
+type progS (i:intS) = STLC.elab_typ i.ct_stlc -> Tot nat
+type ctxS (i:intS) = STLC.elab_typ i.ct_stlc
+type wholeS = (unit -> Tot nat)
+
+let linkS (#i:intS) (ps:progS i) (cs:ctxS i) : wholeS =
+  (fun () -> ps cs)
+
+val behS : wholeS -> propS (STLC.TNat)
+let behS ws = ws ()
+
+(** Target **)
+
+noeq type intT = { ct : STLC.typ }
+
+val comp_int : intS -> intT
+let comp_int i = { ct = i.ct_stlc }
+
+type progT (i:intT) = pt:STLC.exp{STLC.is_value pt} & STLC.typing STLC.empty pt (STLC.TArr i.ct STLC.TNat)
+type ctxT (i:intT) = ct:STLC.exp{STLC.is_value ct} & STLC.typing STLC.empty ct i.ct
+type wholeT = wt:STLC.exp{STLC.is_value wt} & STLC.typing STLC.empty wt (STLC.TArr STLC.TUnit STLC.TNat)
+
+let linkT (#i:intT) (pt:progT i) (ct:ctxT i) : wholeT = 
+  let (| _, htp |) = pt in
+  let (| _, htc |) = ct in
+  let (| ewt, htwt |) = STLC.thunk_exp (STLC.TyApp htp htc) in
+  (| ewt, htwt |)
+
+val behT : wt:wholeT -> propT (STLC.TNat)
+let behT (| ew, htw |) = STLC.eval (STLC.TyApp htw STLC.TyUnit)
+
+(** We can replace the refinement that pt, wt and ct are values,
+    with a refinement that pt, ct and wt can be stepped purely to a value,
+    and then we will need the following lemmas:
+
+assume val pure_step_preserves_behT_wt (wt:wholeT)
+ : Lemma (ensures (
+    ~(STLC.is_value (dfst wt)) /\
+    (forall (wt':wholeT). STLC.pure_step (dfst wt) (dfst wt') ==> 
+      behT wt ≌ behT wt')))
+
+assume val pure_step_preserves_behT_pt #i (pt:progT i) (ct:ctxT i)
+ : Lemma (ensures (
+    ~(STLC.is_value (dfst pt)) /\
+    (forall (pt':progT i). STLC.pure_step (dfst pt) (dfst pt') ==> 
+      behT (linkT pt ct) ≌ behT (linkT pt' ct))))
+
+assume val pure_steps_preserves_behT_wt (wt:wholeT)
+ : Lemma (ensures (
+    forall (wt':wholeT). STLC.pure_steps (dfst wt) (dfst wt') ==> 
+      behT wt ≌ behT wt'))
+
+assume val pure_steps_preserves_behT_pt #i (pt:progT i) (ct:ctxT i)
+ : Lemma (ensures (
+    forall (pt':progT i). STLC.pure_steps (dfst pt) (dfst pt') ==> 
+      behT (linkT pt ct) ≌ behT (linkT pt' ct)))
+**) 
+
+(** Compiler correctness **)
+
+open FStar.Tactics.V2
+open FStar.Reflection.V2
+open FStar.Reflection.Typing
+let mk_squash (phi:term) : Tot term = pack_ln (Tv_App (`squash) (phi, Q_Explicit))
+
+let t_unit = `()
+
+let valid (g:env) (phi:term) : prop =
+  squash (tot_typing g t_unit (mk_squash phi))
+
+let cc (ws:wholeS) (wt:wholeT) =
+  behS ws ≌ behT wt
+
+val compile_whole : 
+  (g:env) ->
+  (ws:term{tot_typing g ws (`wholeS)}) ->
+  Tac (wt:term{
+    tot_typing g wt (`wholeT) /\
+    (** compiler correctness **)
+    valid g (`(cc (`#ws) (`#wt)))
+  })
+(** 
+  If behT is an operational semantics, it has to be small-step because we have external non-determinism.
+  Defining a denotational semantics for STLC is a challenge.
+
+  behS is a denotational semantics.
+
+  Relating the two will be a challenge. Usually, it is really hard to relate denotational and operational semantics
+  of the same language. In this case, we have two different languages, one that it is shallowly embedded and one
+  that is deeply embedded.
+**)
+
+
+// let soundness (#i:intS) (pt:progT (comp_int i)) =
+//   forall (ct:ctxT (comp_int i)). behT (linkT pt ct) ⊆ i.p_post
+
+(** The order of the quantifiers makes this RHC (Robust Hyperproperty Preservation) **)
+let rhc (#i:intS) (ps:progS i) (pt:progT (comp_int i)) =
+  forall (ct:ctxT (comp_int i)).
+    exists (cs:ctxS i). behS (linkS ps cs) ≌ behT (linkT pt ct) 
+
+val backtranslate_ctx : (#i:intS) -> ctxT (comp_int i) -> ctxS i
+let backtranslate_ctx ct = STLC.elab_exp (dsnd ct) STLC.vempty
+
+(** TODO: can we prove RrHP from this since we got rid off the exists? **)
+let rhc_1 (#i:intS) (ps:progS i) (pt:progT (comp_int i)) =
+  forall ct. behS (linkS ps (backtranslate_ctx ct)) ≌ behT (linkT pt ct) 
+
+val compile_prog :
+  (g:env) ->
+  i:term{tot_typing g i (`intS)} ->
+  ps:term{tot_typing g ps (`progS (`#i))} ->
+  Tac (pt:term{
+    tot_typing g pt (`progT (comp_int (`#i))) /\
+
+    (** soundness **)
+    // valid g (`(soundness (`#pt))) /\
+
+    (** RHC **)
+    valid g (`(rhc (`#ps) (`#pt)))
+  })
+
+  // Example of usage:
+  // let i : intS = ...
+  // let ps : progS i = ...
+  // let g_ast : ast_env = ...
+
+  //  %splice_t [pt;pt_sound;ps_pt_rhc] (compile_prog (`i) (`ps) (`g_ast))
+  // // adds in environment the following:
+
+  // let pt : progT (comp_int i g_ast) = ...
+  // let pt_sound : squash (soundness pt) = ...
+  // let ps_pt_rhc : squash (rhc ps pt) = ...
+
+type rel = 
+  #ty:STLC.typ -> 
+  STLC.elab_typ ty ->             (** F* value **)
+  #e:STLC.exp ->                  (** STLC expression **)
+  STLC.typing STLC.empty e ty -> 
+  Type0
+
+(** we want to instantiate this with the result of the compiler,
+    which should give for a ws a wt and a proof of ws `r` wt **)
+let rel_whole (r:rel) (ws:wholeS) (wt:wholeT) : Type0 =
+  ws `r` (dsnd wt) ==> cc ws wt
+
+let rel_pprog (r:rel) i ps pt : Type0 =
+  ps `r` (dsnd pt) ==> rhc_1 #i ps pt
+
+(** Cross-language logical relation,
+    the logical relation is asymmetric because it relates always F* values with STLC's values and expressions *)
+(** Note: usually, this is split into a relation on target values and on target expressions **)
+val (≍) : rel
+let rec (≍) #ty fs_v stlc_ht' =
+  // forall stlc_e', hte', ss:steps stlc_e stlc_e'. is_value stlc_e' ==>
+  (** First, we make sure that stlc_e contains a value. (fst_e is already a value)**)
+  let (| stlc_e, stlc_ht |) = STLC.eval stlc_ht' in (** it is ok to use eval when it means a big-step operational semantics
+                                                       and not an interpreter (in the longer run) **)
+  // assert (STLC.is_value stlc_e);
+  match stlc_ht with
+  // base types
+  | STLC.TyUnit
+  | STLC.TyZero
+  | STLC.TySucc _ ->
+    (** One can avoid using elab_exp, but using it simplifies proofs later **)
+    fs_v ∽ stlc_ht
+  
+  // polymorphic types
+  | STLC.TyInl #_ #_ #t1 t2 ht1 ->
+    let fst_inl : either (STLC.elab_typ t1) (STLC.elab_typ t2) = fs_v in
+    Inl? fst_inl /\ (Inl?.v fst_inl ≍ ht1)
+  | STLC.TyInr #_ #_ t1 #t2 ht2 ->
+    let fs_inr : either (STLC.elab_typ t1) (STLC.elab_typ t2) = fs_v in
+    Inr? fs_inr /\ (Inr?.v fs_inr ≍ ht2)
+  | STLC.TyPair #_ #_ #_ #t1 #t2 ht_fst ht_snd ->
+    let (fs_fst, fs_snd) : (STLC.elab_typ t1 * STLC.elab_typ t2) = fs_v in
+    (fs_fst ≍ ht_fst) /\ (fs_snd ≍ ht_snd)
+
+  // lambda
+  | STLC.TyLam tv #_ #t' _ -> 
+    let fs_f : STLC.elab_typ tv -> STLC.elab_typ t' = fs_v in
+    forall stlc_x (ht_x:STLC.typing STLC.empty stlc_x tv). (** all values possible in STLC **)
+      forall fs_x.
+      // let fst_v = STLC.elab_exp htv STLC.vempty in (** this is non-standard, and it may produce problems in HO cases **)
+        (fs_x ≍ ht_x) ==> ((fs_f fs_x) ≍ (STLC.TyApp stlc_ht ht_x))
+
+let x1 : STLC.exp =
+    STLC.ELam STLC.TNat (STLC.EVar 0)
+let x1ty : STLC.typing STLC.empty x1 (STLC.TArr STLC.TNat STLC.TNat) =
+    STLC.TyLam STLC.TNat (STLC.TyVar 0)
+
+let test123 =
+  assert ((fun (x:nat) -> x) ≍ x1ty) by (compute ())
+
+// let x2 : STLC.exp =
+//     STLC.ELam STLC.TNat (STLC.ELam STLC.TUnit (STLC.EVar 1))
+// let x2ty : STLC.typing STLC.empty x2 (STLC.TArr STLC.TNat (STLC.TArr STLC.TUnit STLC.TNat)) =
+//     STLC.TyLam STLC.TNat (STLC.TyLam STLC.TUnit (STLC.TyVar 1))
+
+// let test1234 =
+//   assert ((fun (x:nat) -> (fun () -> x)) ≍ x2ty) by (
+//       compute ();
+//       explode ();
+//       dump "H"
+//   )
+
+(** we don't really need this since F* can figure it out by itself, but
+    it is useful to keep track where it is used. If we change the refinement
+    on pt, ct and wt, then we will need to replace it. **)
+let eval_value_is_id (#e:STLC.exp) (#t:STLC.typ) (ht:STLC.typing STLC.empty e t)
+  : Lemma (STLC.is_value e ==> STLC.eval ht == (| e, ht |)) = ()
+
+let rel_implies_cc ws wt : Lemma (rel_whole (≍) ws wt) = 
+  let (| ew, htw |) = wt in
+  introduce 
+    ws ≍ (dsnd wt)
+  ==> 
+    behS ws ≌ behT wt
+  with _. begin
+    assert (ws ≍ htw);
+    // unfolding ≍
+    let (| ewt', htwt' |) = STLC.eval htw in
+    assert (ws ≍ htwt'); // wt' is a value (Lam) and returns a nat
+    assert (behS ws ≌ behT (| ewt', htwt' |));
+    eval_value_is_id htw;
+    assert (behT (| ewt', htwt' |) == behT wt);
+    assert (behS ws ≌ behT wt)
+  end
+
+val elab_rel (#e:STLC.exp) (#t:STLC.typ) (ht:STLC.typing STLC.empty e t)
+  : Lemma (STLC.elab_exp ht STLC.vempty ≍ ht)
+let rec elab_rel #e #t ht =
+  match ht with
+  | STLC.TyUnit -> ()
+  | STLC.TyZero -> ()
+  | STLC.TySucc _ -> admit ()
+  | STLC.TyApp h1 h2 -> admit ()
+  | _ -> admit ()
+
+let rel_implies_rhc i ps pt : Lemma (rel_pprog (≍) i ps pt) = 
+  introduce 
+    ps ≍ (dsnd pt)
+  ==> 
+    (forall ct. behS (linkS ps (backtranslate_ctx ct)) ≌ behT (linkT pt ct) )
+  with _. begin
+    introduce 
+      forall ct. behS (linkS ps (backtranslate_ctx ct)) ≌ behT (linkT pt ct)
+    with begin
+      // unfolding ≍
+      let (| ept', htpt' |) = STLC.eval (dsnd pt) in
+      eval_value_is_id (dsnd pt);
+      assert (behT (linkT pt ct) == behT (linkT (| ept', htpt' |) ct));
+
+      // ps ≍ (dsnd pt) implies:
+      assert (ps ≍ htpt');
+      
+      let cs = backtranslate_ctx ct in
+      elab_rel (dsnd ct);
+      assert (cs ≍ dsnd ct);
+
+      let htbody = STLC.TyApp htpt' (dsnd ct) in
+      assert (ps cs ≍ htbody);
+
+      let (| ewt, htwt |) = STLC.thunk_exp htbody in
+      let htwtapp = STLC.TyApp htwt STLC.TyUnit in
+      assume (ps cs ≍ htwtapp); // this should be simple to prove
+
+      assert (behS (linkS ps cs) ≌ behT (linkT (| ept', htpt' |) ct));
+      assert (behS (linkS ps cs) ≌ behT (linkT pt ct))
+    end
+  end
+
+
+    //  (EInl? e && is_value (EInl?.v e)) ||
+    //  (EInr? e && is_value (EInr?.v e)) || 
+    //  EByteLit? e || 
+    //  (EPair? e && is_value (EPair?.fst e) && is_value (EPair?.snd e) ) || 
+    //  (EBytesCreate? e && is_value (EBytesCreate?.v e) && is_value (EBytesCreate?.n e)) || (* TODO: this is kind of weird, but we don't have enough syntax to interpret this *)
+    //  EStringLit? e
