meta/STLC.fst
@@ -1,0 +1,825 @@
+(* Based on file FStar/examples/metatheory/StlcStrongDbParSubst.fst *)
+
+module STLC
+
+open FStar.Tactics
+open FStar.Constructive
+open FStar.Classical
+open FStar.FunctionalExtensionality
+
+(* Constructive-style progress and preservation proof for STLC with
+   strong reduction, using deBruijn indices and parallel substitution. *)
+
+type typ =
+  | TArr    : typ -> typ -> typ
+  | TSum    : typ -> typ -> typ
+  | TPair   : typ -> typ -> typ
+  | TUnit   : typ
+  | TNat    : typ
+//   | TByte   : typ
+//   | TBytes  : typ
+//   | TExn    : typ
+//   | TFDesc  : typ
+//   | TString : typ
+
+let rec is_fo_typ (t:typ) =
+  match t with
+  | TUnit -> True
+  | TNat -> True
+  | TPair t1 t2 -> is_fo_typ t1 /\ is_fo_typ t2
+  | TSum t1 t2 -> is_fo_typ t1 /\ is_fo_typ t2
+  | TArr _ _ -> False
+
+type fo_typ = t:typ{is_fo_typ t}
+
+type var = nat
+
+open FStar.Bytes
+
+type exp =
+  | EVar         : var -> exp
+  | EApp         : exp -> exp -> exp
+  | ELam         : typ -> exp -> exp
+  | EUnit        : exp
+  | EZero        : exp
+  | ESucc        : v:exp -> exp
+  | ENRec        : exp -> exp -> exp -> exp
+  | EInl         : v:exp -> exp
+  | EInr         : v:exp -> exp
+  | ECase        : exp -> exp -> exp -> exp
+//   | EByteLit     : byte -> exp
+//   | EBytesCreate : n:exp -> v:exp -> exp
+  | EFst         : exp -> exp
+  | ESnd         : exp -> exp
+  | EPair        : fst:exp -> snd:exp -> exp
+//   | EStringLit   : v:string -> exp
+
+
+(* Type system; as inductive relation (not strictly necessary for STLC) *)
+
+type env = var -> Tot (option typ)
+
+val empty : env
+let empty _ = None
+
+(* we only need extend at 0 *)
+val extend : typ -> env -> Tot env
+let extend t g y = if y = 0 then Some t
+                   else g (y-1)
+
+noeq type typing : env -> exp -> typ -> Type =
+  | TyVar : #g:env ->
+             x:var{Some? (g x)} ->
+             typing g (EVar x) (Some?.v (g x))
+  | TyLam : #g :env ->
+             t :typ ->
+            #e1:exp ->
+            #t':typ ->
+            $hbody:typing (extend t g) e1 t' ->
+                   typing g (ELam t e1) (TArr t t')
+  | TyApp : #g:env ->
+            #e1:exp ->
+            #e2:exp ->
+            #t11:typ ->
+            #t12:typ ->
+            $h1:typing g e1 (TArr t11 t12) ->
+            $h2:typing g e2 t11 ->
+                typing g (EApp e1 e2) t12
+  | TyUnit : #g:env ->
+             typing g EUnit TUnit
+  | TyZero : #g:env ->
+             typing g EZero TNat
+  | TySucc : #g:env ->
+             #e:exp ->
+             $h1:typing g e TNat ->
+                 typing g (ESucc e) TNat
+  | TyNRec : #g:env ->
+             #e1:exp ->
+             #e2:exp ->
+             #e3:exp ->
+             #t1:typ ->
+             $h1:typing g e1 TNat ->
+             $h2:typing g e2 t1 ->
+             $h3:typing g e3 (TArr t1 t1) ->
+                 typing g (ENRec e1 e2 e3) t1
+  | TyInl  : #g:env ->
+             #e:exp ->
+             #t1:typ ->
+             t2:typ ->
+             $h1:typing g e t1 ->
+                 typing g (EInl e) (TSum t1 t2)
+  | TyInr  : #g:env ->
+             #e:exp ->
+             t1:typ ->
+             #t2:typ ->
+             $h1:typing g e t2 ->
+                 typing g (EInr e) (TSum t1 t2)
+  | TyCase : #g:env ->
+             #e1:exp ->
+             #e2:exp ->
+             #e3:exp ->
+             #t1:typ ->
+             #t2:typ ->
+             #t3:typ ->
+             $h1:typing g e1 (TSum t1 t2) ->
+             $h2:typing g e2 (TArr t1 t3) ->
+             $h3:typing g e3 (TArr t2 t3) ->
+                 typing g (ECase e1 e2 e3) t3
+//   | TyByteLit : #g:env ->
+//                 b:byte ->
+//                    typing g (EByteLit b) TByte
+//   | TyBytesCreate : #g:env ->
+//                     #e1:exp ->
+//                     #e2:exp ->
+//                     $h1:typing g e1 TNat ->
+//                     $h2:typing g e2 TByte ->
+//                         typing g (EBytesCreate e1 e2) TBytes
+  | TyFst         : #g:env ->
+                    #e:exp ->
+                    #t1:typ ->
+                    #t2:typ ->
+                    $h1:typing g e (TPair t1 t2) ->
+                        typing g (EFst e) t1
+  | TySnd         : #g:env ->
+                    #e:exp ->
+                    #t1:typ ->
+                    #t2:typ ->
+                    $h1:typing g e (TPair t1 t2) ->
+                        typing g (ESnd e) t2
+  | TyPair        : #g:env ->
+                    #e1:exp ->
+                    #e2:exp ->
+                    #t1:typ ->
+                    #t2:typ ->
+                    $h1:typing g e1 t1 ->
+                    $h2:typing g e2 t2 ->
+                        typing g (EPair e1 e2) (TPair t1 t2)
+//   | TyStringLit   : #g:env ->
+//                     s:string ->
+//                        typing g (EStringLit s) TString
+
+(* Parallel substitution operation `subst` *)
+
+(* The termination argument uses a lexicographic ordering composed of:
+   0) a bit saying whether the expression is a variable or not;
+   1) an _undecidable_ well-founded order on substitutions that
+      equates all renamings, equates all non-renamings, and makes
+      renamings strictly smaller than non-renamings; we write down a
+      non-constructive function is_renaming mapping substitutions
+      (infinite objects) to 0 (renaming) or 1 (non-renaming)
+   2) the structure of the expression e *)
+
+(* Parallel substitution operation `subst` *)
+let sub (renaming:bool) = 
+    f:(var -> exp){ renaming <==> (forall x. EVar? (f x)) }
+
+let bool_order (b:bool) = if b then 0 else 1
+
+let sub_inc 
+  : sub true
+  = fun y -> EVar (y+1)
+
+let is_var (e:exp) : int = if EVar? e then 0 else 1
+
+let rec subst (#r:bool)
+              (s:sub r)
+              (e:exp)
+  : Tot (e':exp { r ==> (EVar? e <==> EVar? e') })
+        (decreases %[bool_order (EVar? e); 
+                     bool_order r;
+                     1;
+                     e])
+  = match e with
+  | EVar x -> s x
+  | ELam t e1 -> ELam t (subst (sub_elam s) e1)
+  | EApp e1 e2 -> EApp (subst s e1) (subst s e2)
+  | EUnit -> EUnit
+  | EZero -> EZero
+  | ESucc e -> ESucc (subst s e)
+  | ENRec e1 e2 e3 -> ENRec (subst s e1) (subst s e2) (subst s e3)
+  | EInl e -> EInl (subst s e)
+  | EInr e -> EInr (subst s e)
+  | ECase e1 e2 e3 -> ECase (subst s e1) (subst s e2) (subst s e3)
+//   | EByteLit b -> EByteLit b
+//   | EBytesCreate e1 e2 -> EBytesCreate (subst s e1) (subst s e2)
+  | EFst e -> EFst (subst s e)
+  | ESnd e -> ESnd (subst s e)
+  | EPair e1 e2 -> EPair (subst s e1) (subst s e2)
+//   | EStringLit s -> EStringLit s
+
+and sub_elam (#r:bool) (s:sub r) 
+  : Tot (sub r)
+        (decreases %[1;
+                     bool_order r;
+                     0;
+                     EVar 0])
+  = let f : var -> exp = 
+      fun y ->
+        if y=0
+        then EVar y
+        else subst sub_inc (s (y - 1))
+    in
+    introduce not r ==> (exists x. ~ (EVar? (f x)))
+    with not_r. 
+      eliminate exists y. ~ (EVar? (s y))
+      returns (exists x. ~ (EVar? (f x)))
+      with (not_evar_sy:squash (~(EVar? (s y)))). 
+        introduce exists x. ~(EVar? (f x))
+        with (y + 1)
+        and ()
+    ;
+    f
+
+let sub_beta (e:exp)
+  : sub (EVar? e)
+  = let f = 
+      fun (y:var) ->
+        if y = 0 then e      (* substitute *)
+        else (EVar (y-1))    (* shift -1 *)
+    in
+    if not (EVar? e)
+    then introduce exists (x:var). ~(EVar? (f x))
+         with 0 and ();
+    f
+
+(* Small-step operational semantics; strong / full-beta reduction is
+   non-deterministic, so necessarily as inductive relation *)
+
+type pure_step : exp -> exp -> Type =
+  | SBeta : t:typ ->
+            e1:exp ->
+            e2:exp ->
+            pure_step (EApp (ELam t e1) e2) (subst (sub_beta e2) e1)
+  | SApp1 : #e1:exp ->
+             e2:exp ->
+            #e1':exp ->
+            $hst:pure_step e1 e1' ->
+                 pure_step (EApp e1 e2) (EApp e1' e2)
+  | SApp2 :   e1:exp ->
+             #e2:exp ->
+            #e2':exp ->
+            $hst:pure_step e2 e2' ->
+                 pure_step (EApp e1 e2) (EApp e1 e2')
+  | SSucc :    e:exp ->
+             #e':exp ->
+            $hst:pure_step e e' ->
+                 pure_step (ESucc e) (ESucc e')     
+  | SNRecV :  #e1:exp ->
+             #e1':exp ->
+               e2:exp ->
+               e3:exp ->
+             $hst:pure_step e1 e1' ->
+                 pure_step (ENRec e1 e2 e3) (ENRec e1' e2 e3)
+//   | SNRecX :   e1:exp ->
+//                e2:exp ->
+//              #e2':exp ->
+//                e3:exp ->
+//              $hst:pure_step e2 e2' ->
+//                  pure_step (ENRec e1 e2 e3) (ENRec e1 e2' e3)                 
+  | SNRec0 : e2:exp ->
+             e3:exp ->
+                 pure_step (ENRec EZero e2 e3) e2
+  | SNRecIter :  v:exp ->
+                e2:exp ->
+                e3:exp ->
+                pure_step (ENRec (ESucc v) e2 e3) (ENRec v (EApp e3 e2) e3)
+  | SInl  :    e:exp ->
+             #e':exp ->
+            $hst:pure_step e e' ->
+                 pure_step (EInl e) (EInl e')
+  | SInr  :    e:exp ->
+             #e':exp ->
+            $hst:pure_step e e' ->
+                 pure_step (EInr e) (EInr e')
+  | SCase :  #e1:exp ->
+            #e1':exp ->
+              e2:exp ->
+              e3:exp ->
+            $hst:pure_step e1 e1' ->
+                 pure_step (ECase e1 e2 e3) (ECase e1' e2 e3)
+  | SCaseInl :  v:exp ->
+               e2:exp ->
+               e3:exp ->
+                 pure_step (ECase (EInl v) e2 e3) (EApp e2 v)
+  | SCaseInr :  v:exp ->
+               e2:exp ->
+               e3:exp ->
+                 pure_step (ECase (EInr v) e2 e3) (EApp e3 v)
+  | SFst0 :    #e:exp ->
+              #e':exp ->
+             $hst:pure_step e e' ->
+                 pure_step (EFst e) (EFst e')
+  | SFst :  e1:exp ->
+            e2:exp ->
+               pure_step (EFst (EPair e1 e2)) e1
+  | SSnd0 :    #e:exp ->
+              #e':exp ->
+             $hst:pure_step e e' ->
+                 pure_step (ESnd e) (ESnd e')
+  | SSnd :  e1:exp ->
+            e2:exp ->
+               pure_step (ESnd (EPair e1 e2)) e2
+  | SPair1  : #e1:exp ->
+             #e1':exp ->
+             $hst:pure_step e1 e1' ->
+               e2:exp ->
+                 pure_step (EPair e1 e2) (EPair e1' e2)
+  | SPair2  :  e1:exp ->
+              #e2:exp ->
+             #e2':exp ->
+             $hst:pure_step e2 e2' ->
+                 pure_step (EPair e1 e2) (EPair e1 e2')
+//   | SBytesCreateN : #e1:exp ->
+//                    #e1':exp ->
+//                    e2:exp ->
+//                    $hst:pure_step e1 e1' ->
+//                    pure_step (EBytesCreate e1 e2) (EBytesCreate e1' e2)
+//   | SBytesCreateV : e1:exp ->
+//                    #e2:exp ->
+//                    #e2':exp ->
+//                    $hst:pure_step e2 e2' ->
+//                    pure_step (EBytesCreate e1 e2) (EBytesCreate e1 e2')
+
+type step = pure_step
+
+type pure_steps : exp -> exp -> Type =
+  | PSrefl   : e:exp ->
+               pure_steps e e
+  | PSMany   : #e1:exp ->
+               #e2:exp ->
+               #e3:exp ->
+               $hst:pure_step e1 e2 ->
+               $hsts:pure_steps e2 e3 ->
+               pure_steps e1 e3
+
+type steps : exp -> exp -> Type =
+  | Srefl  : e:exp ->
+             steps e e
+  | SMany   : #e1:exp ->
+              #e2:exp ->
+              #e3:exp ->
+              $hst:step e1 e2 ->
+              $hsts:steps e2 e3 ->
+              steps e1 e3
+
+let rec is_value (e:exp) : bool = 
+     match e with
+     | ELam _  _
+     | EUnit 
+     | EZero -> true
+     | ESucc e -> is_value e
+     | EInl e -> is_value e
+     | EInr e -> is_value e 
+     | EPair e1 e2 -> is_value e1 && is_value e2
+     | _ -> false
+     // EByteLit? e || 
+     // (EBytesCreate? e && is_value (EBytesCreate?.v e) && is_value (EBytesCreate?.n e)) || (* TODO: this is kind of weird, but we don't have enough syntax to interpret this *)
+     // EStringLit? e
+
+let rec progress (#e:exp { ~(is_value e) })
+                 (#t:typ)
+                 (h:typing empty e t)
+  : e':exp & step e e'
+  =  match h with
+     | TyApp #g #e1 #e2 #t11 #t12 h1 h2 -> 
+     begin
+          match e1 with
+          | ELam t e1' -> (| subst (sub_beta e2) e1', SBeta t e1' e2 |)
+          | _          -> let (| e1', h1' |) = progress h1 in
+                              (| EApp e1' e2, SApp1 e2 h1'|) (** TODO: call-by-name **)
+     end
+     | TySucc #g #e h1 ->
+          let (| e', h1' |) = progress h1 in
+          (| ESucc e', SSucc e h1'|)
+     | TyNRec #g #e1 #e2 #e3 #t1 h1 h2 h3 -> begin
+          match e1 with
+          | EZero -> (| e2, SNRec0 e2 e3 |)
+          | ESucc v -> (| ENRec v (EApp e3 e2) e3, SNRecIter v e2 e3 |)
+          | _ -> let (| e1', h1' |) = progress h1 in
+                 (| ENRec e1' e2 e3, SNRecV e2 e3 h1' |)
+     end
+     | TyInl #g #e #t1 #t2 h1 -> 
+          let (| e', h1' |) = progress h1 in
+          (| EInl e', SInl e h1'|)
+     | TyInr #g #e #t1 #t2 h1 -> 
+          let (| e', h1' |) = progress h1 in
+          (| EInr e', SInr e h1'|)
+     | TyCase #g #e1 #e2 #e3 #t1 #t2 #t3 h1 h2 h3 -> begin
+          match e1 with
+          | EInl v -> (| EApp e2 v, SCaseInl v e2 e3 |)
+          | EInr v -> (| EApp e3 v, SCaseInr v e2 e3 |)
+          | _ ->
+               let (| e1', h1' |) = progress h1 in
+               (| ECase e1' e2 e3, SCase e2 e3 h1' |)
+     end
+     | TyFst #g #e #t1 #t2 h1 -> begin
+          match e with
+          | EPair e1 e2 -> (| e1, SFst e1 e2 |)
+          | _ -> let (| e', h1' |) = progress h1 in
+                 (| EFst e', SFst0 h1' |)
+     end
+     | TySnd #g #e #t1 #t2 h1 -> begin
+          match e with
+          | EPair e1 e2 -> (| e2, SSnd e1 e2 |)
+          | _ -> let (| e', h1' |) = progress h1 in
+                 (| ESnd e', SSnd0 h1' |)
+     end
+     | TyPair #g #e1 #e2 #t1 #t2 h1 h2 -> 
+          if is_value e1 then
+               let (| e2', h2' |) = progress h2 in
+               (| EPair e1 e2', SPair2 e1 h2' |)
+          else 
+               let (| e1', h1' |) = progress h1 in
+               (| EPair e1' e2, SPair1 h1' e2 |)
+     // | TyBytesCreate #g #e1 #e2 h1 h2 -> begin
+     //      if is_value e1 then
+     //           let (| e2', h2' |) = progress h2 in
+     //           (| EBytesCreate e1 e2', SBytesCreateV e1 h2' |)
+     //      else 
+     //           let (| e1', h1' |) = progress h1 in
+     //           (| EBytesCreate e1' e2, SBytesCreateN e2 h1' |)
+     // end
+
+
+(* Typing of substitutions (very easy, actually) *)
+let subst_typing #r (s:sub r) (g1:env) (g2:env) =
+    x:var{Some? (g1 x)} -> typing g2 (s x) (Some?.v (g1 x))
+
+(* Substitution preserves typing
+   Strongest possible statement; suggested by Steven Schäfer *)
+let rec substitution (#g1:env) 
+                     (#e:exp)
+                     (#t:typ)
+                     (#r:bool)
+                     (s:sub r)
+                     (#g2:env)
+                     (h1:typing g1 e t)
+                     (hs:subst_typing s g1 g2)
+   : Tot (typing g2 (subst s e) t)
+         (decreases %[bool_order (EVar? e); bool_order r; e])
+   = match h1 with
+   | TyVar x -> hs x
+   | TyLam tlam hbody ->
+     let hs'' : subst_typing (sub_inc) g2 (extend tlam g2) =
+       fun x -> TyVar (x+1) in
+     let hs' : subst_typing (sub_elam s) (extend tlam g1) (extend tlam g2) =
+       fun y -> if y = 0 then TyVar y
+             else substitution sub_inc (hs (y - 1)) hs''
+     in TyLam tlam (substitution (sub_elam s) hbody hs')
+      | TyApp hfun harg -> TyApp (substitution s hfun hs) (substitution s harg hs)
+   | TyUnit -> TyUnit
+   | TyZero -> TyZero
+   | TySucc h1 -> TySucc (substitution s h1 hs)
+   | TyNRec h1 h2 h3 -> TyNRec (substitution s h1 hs) (substitution s h2 hs) (substitution s h3 hs)
+   | TyInl t2 h1 -> 
+     let EInl e' = e in
+     let hs' : typing g2 (EInl (subst s e')) t = TyInl t2 (substitution s h1 hs) in
+     assert (subst s e == EInl (subst s e'));
+     hs'
+   | TyInr t1 h1 -> 
+     let EInr e' = e in
+     let hs' : typing g2 (EInr (subst s e')) t = TyInr t1 (substitution s h1 hs) in
+     assert (subst s e == EInr (subst s e'));
+     hs'
+   | TyCase h1 h2 h3 -> TyCase (substitution s h1 hs) (substitution s h2 hs) (substitution s h3 hs)
+   | TyFst h1 -> TyFst (substitution s h1 hs)
+   | TySnd h1 -> TySnd (substitution s h1 hs)
+   | TyPair h1 h2 -> TyPair (substitution s h1 hs) (substitution s h2 hs)
+//    | TyByteLit b -> TyByteLit b
+//    | TyBytesCreate h1 h2 -> TyBytesCreate (substitution s h1 hs) (substitution s h2 hs)
+//    | TyStringLit s -> TyStringLit s
+
+(* Substitution for beta reduction
+   Now just a special case of substitution lemma *)
+let substitution_beta #e #v #t_x #t #g 
+                      (h1:typing g v t_x)
+                      (h2:typing (extend t_x g) e t)
+  : typing g (subst (sub_beta v) e) t
+  = let hs : subst_typing (sub_beta v) (extend t_x g) g =
+        fun y -> if y = 0 then h1 else TyVar (y-1) in
+    substitution (sub_beta v) h2 hs
+
+
+(* Type preservation *)
+let rec preservation_step #e #e' #g #t (ht:typing g e t) (hs:step e e') 
+  : typing g e' t
+  =  match hs with
+     | SBeta tx e1' e2' -> 
+          let TyApp h1 h2 = ht in
+          substitution_beta h2 (TyLam?.hbody h1)
+     | SApp1 e2' hs1   -> 
+          let TyApp h1 h2 = ht in
+          TyApp (preservation_step h1 hs1) h2
+     | SApp2 e1' hs2   -> 
+          let TyApp h1 h2 = ht in
+          TyApp h1 (preservation_step h2 hs2)
+     | SSucc e' hs1    -> 
+          let TySucc h1 = ht in
+          TySucc (preservation_step h1 hs1)
+     | SNRecV _ _ hs1 ->
+          let TyNRec h1 h2 h3 = ht in
+          TyNRec (preservation_step h1 hs1) h2 h3
+     | SNRec0 _ _ ->
+          let TyNRec h1 h2 h3 = ht in
+          h2
+     | SNRecIter _ _ _ ->
+          // assert (e == ENRec (ESucc v) e2' e3');
+          // assert (e' == ENRec v (EApp e3' e2') e3');
+          let TyNRec h1 h2 h3 = ht in
+          let TySucc h1' = h1 in
+          TyNRec h1' (TyApp h3 h2) h3
+     | SInl _ hs1     -> 
+          let TyInl t2 h1 = ht in
+          TyInl t2 (preservation_step h1 hs1)
+     | SInr _ hs1     -> 
+          let TyInr t1 h1 = ht in
+          TyInr t1 (preservation_step h1 hs1)
+     | SCase _ _ hs1 -> 
+          let TyCase h1 h2 h3 = ht in
+          TyCase (preservation_step h1 hs1) h2 h3
+     | SCaseInl _ _ _ -> 
+          let TyCase h1 h2 h3 = ht in
+          let TyInl _ h1' = h1 in
+          TyApp h2 h1'
+     | SCaseInr _ _ _ -> 
+          let TyCase h1 h2 h3 = ht in
+          let TyInr _ h1' = h1 in
+          TyApp h3 h1'
+     | SFst0 hs1 -> 
+          let TyFst h1 = ht in
+          TyFst (preservation_step h1 hs1)
+     | SFst _ _ -> 
+          let TyFst h1 = ht in
+          let TyPair h1' _ = h1 in
+          h1'
+     | SSnd0 hs1 -> 
+          let TySnd h1 = ht in
+          TySnd (preservation_step h1 hs1)
+     | SSnd _ _ -> 
+          let TySnd h1 = ht in
+          let TyPair _ h1' = h1 in
+          h1'
+     | SPair1 hs1 _ ->
+          let TyPair h1 h2 = ht in
+          TyPair (preservation_step h1 hs1) h2
+     | SPair2 _ hs2 ->
+          let TyPair h1 h2 = ht in
+          TyPair h1 (preservation_step h2 hs2)
+     // | SBytesCreateN _ hs1 ->
+     //      let TyBytesCreate h1 h2 = ht in
+     //      TyBytesCreate (preservation_step h1 hs1) h2
+     // | SBytesCreateV _ hs2 ->
+     //      let TyBytesCreate h1 h2 = ht in
+     //      TyBytesCreate h1 (preservation_step h2 hs2)
+
+// let (+*) (x:int) (y:int) : int = Prims.op_Multiply x y
+// let rec (^) (x:nat) (y:nat) : Tot (r:nat{x > 0 ==> r > 0}) (decreases y)=
+//      if y = 0 then 1 else x +* (x ^ (y-1))
+
+// (** ** Evaluation *)
+// let rec weight (e:exp) : (r:nat{r > 0}) =
+//      match e with
+//      | EVar x -> 1
+//      | EApp e1 e2 -> weight e1 +* weight e2
+//      | ELam _ e1 -> 1 + weight e1
+//      | EUnit -> 1
+//      | EZero -> 1
+//      | ESucc e -> 1 + weight e
+//      | ENRec e1 e2 e3 -> (1 + weight e2) +* ((weight e3) ^ weight e1)
+//      | EInl e -> 1 + weight e
+//      | EInr e -> 1 + weight e
+//      | ECase e1 e2 e3 -> 1 + weight e1 + weight e2 + weight e3
+//      | EByteLit _ -> 1
+//      | EBytesCreate e1 e2 -> 1 + weight e1 + weight e2
+//      | EFst e -> 1 + weight e
+//      | ESnd e -> 1 + weight e
+//      | EPair e1 e2 -> 1 + weight e1 + weight e2
+//      | EStringLit _ -> 1
+
+// #set-options "--print_implicits"
+
+// let distribute_multiply x y z : Lemma ((x + y) +* z = x +* z + (y +* z)) = ()
+// let fold_multiply_power x n : Lemma (x +* (x^n) == x^(n+1)) = ()
+// let rec power_less (x:nat{x > 1}) (n:nat) : Lemma ((x^(n+1)) > x^n) =
+//      match n with
+//      | 0 -> ()
+//      | _ -> power_less (x) (n-1)
+
+// let rec step_decreases_weight #g (#e:exp) (#e':exp) #t (ht:typing g e t) (hs:step e e')
+//   : Lemma (weight e' < weight e) 
+//   =  assume (forall x y z. x < y ==> x +* z < y +* z);
+//      assume (forall x z. z +* x == x +* z);
+//      match hs with
+//      | SBeta t e1 e2 -> admit ()
+//           // assert (e == (EApp (ELam t e1) e2));
+//           // assert (e' == subst (sub_beta e2) e1);
+//           // assume (weight (subst (sub_beta e2) e1) < weight e)
+//     | SApp1 #e1 e2 #e1' hs1 -> 
+//           let TyApp ht1 _ = ht in
+//           step_decreases_weight ht1 hs1
+//      | SApp2 e1 #e2 #e2' hs2 -> 
+//           let TyApp _ ht2 = ht in
+//           step_decreases_weight ht2 hs2
+//      | SSucc e1 #e' hs1 ->
+//           let TySucc ht1 = ht in
+//           step_decreases_weight ht1 hs1
+// //      | SNRecV #e1 #e1' e2 e3 hs1 ->
+// //           let TyNRec ht1 ht2 ht3 = ht in
+// //           step_decreases_weight ht1 hs1
+// //      | SNRec0 e2 e3 -> admit ()
+//           // let TyNRec ht1 ht2 ht3 = ht in
+//           // let TyLam _ _ : typing g e3 (TArr _ _) = ht3 in
+//           // assert (ELam? e3);
+//           // assert (weight e3 > 1);
+//           // ()
+//        | SNRecIter v e2 e3 ->
+//           let TyNRec htv ht2 ht3 = ht in
+//           // let TyLam _ _ : typing g e3 (TArr _ _) = ht3 in
+//           assume (ELam? e3); // inversion lemma needed
+//           assert (weight e3 > 1);
+//           calc (>) {
+//                weight e <: int;
+//                == {}
+//                weight (ENRec (ESucc v) e2 e3) <: int;
+//                == {}
+//                (1 + weight e2) +* ((weight e3) ^ weight (ESucc v));
+//                == {}
+//                (1 + weight e2) +* ((weight e3) ^ (weight v + 1));
+//                == { distribute_multiply 1 (weight e2) ((weight e3) ^ (weight v + 1)) }
+//                ((weight e3) ^ (weight v + 1)) + (weight e2 +* ((weight e3) ^ (weight v + 1)));
+//                > { power_less (weight e3) (weight v) }
+//                ((weight e3) ^ weight v) + (weight e2 +* ((weight e3) ^ (weight v + 1)));
+//                == { fold_multiply_power (weight e3) (weight v) } // fold x * x^n to x^(n+1)
+//                ((weight e3) ^ weight v) + (weight e2 +* (weight e3 +* ((weight e3) ^ weight v)));
+//                == { _ by (tadmit ()) (** assoc **) } // reorder multiplication
+//                ((weight e3) ^ weight v) + ((weight e3 +* weight e2) +* ((weight e3) ^ weight v));
+//                == { distribute_multiply 1 (weight e3 +* weight e2) ((weight e3) ^ weight v) }
+//                (1 + (weight e3 +* weight e2)) +* ((weight e3) ^ weight v);
+//                == {} // unfold weight EApp
+//                (1 + (weight (EApp e3 e2))) +* ((weight e3) ^ weight v);
+//                == {} // unfold weight once
+//                weight (ENRec v (EApp e3 e2) e3) <: int;
+//                == {}
+//                weight e' <: int;
+//           }
+//      | _ -> admit ()
+
+// using from Software Foundations, the proof that norm halts using a logical relation,
+// we can make eval return the steps
+// and then define a size to count the number of steps,
+// and then prove that the size decreases in each step:
+//   t --> t' => size (eval t) > size (eval t')  !!! Problem: recursive definition
+
+(** Phil Wadler: Progress + Preservation = Evaluation. **)
+let eval_step #e #t 
+              (ht:typing empty e t) 
+  : either (squash (is_value e))
+           (e':exp & step e e' & typing empty e' t)
+  = if is_value e then Inl ()
+    else let (| e', s |) = progress ht in
+         let ht' = preservation_step ht s in
+         Inr (| e', s, ht' |)
+
+let rec eval (#e:exp) (#t:typ) (ht:typing empty e t)
+  : Tot (e':exp{is_value e'} & typing empty e' t)
+  = match eval_step ht with
+    | Inl _ -> (| e, ht |)
+    | Inr (| _, _, ht' |) -> 
+          admit (); (** TODO: proof of termination required **)
+          eval ht'
+
+(** *** Elaboration of types and expressions to F* *)
+
+open FStar.Ghost
+open FStar.UInt32
+let convert (n : nat) : u32 = if n < 65535 then (uint_to_t n <: u32) else 0ul
+
+type file_descr = int
+
+let rec elab_typ (t:typ) : Type =
+  match t with
+  | TArr t1 t2 -> (elab_typ t1) -> Tot (elab_typ t2)
+  | TUnit -> unit
+  | TNat -> nat
+  | TSum t1 t2 -> either (elab_typ t1) (elab_typ t2)
+  | TPair t1 t2 -> (elab_typ t1) * (elab_typ t2)
+//   | TByte -> byte
+//   | TBytes -> bytes
+//   | TExn -> exn
+//   | TFDesc -> file_descr
+//   | TString -> string
+
+
+type venv (g:env) = x:var{Some? (g x)} -> elab_typ (Some?.v (g x))
+
+let vempty : venv empty = fun _ -> assert false
+
+let vextend #t (x:elab_typ t) (#g:env) (ve:venv g) : venv (extend t g) =
+  fun y -> if y = 0 then x else ve (y-1)
+
+let cast_TArr #t1 #t2 (h : (elab_typ t1 -> Tot (elab_typ t2))) : elab_typ (TArr t1 t2) = h
+
+open FStar.List.Tot
+
+let rec fnrec (#a:Type) (n:nat) (acc:a) (iter:a -> a): Tot a =
+     if n = 0 then acc else fnrec (n-1) (iter acc) iter
+
+let rec elab_exp (#g:env) (#e:exp) (#t:typ) (h:typing g e t) (ve:venv g)
+  : Tot (elab_typ t) (decreases e) =
+  match h with
+  | TyUnit -> ()
+  | TyZero -> 0
+  | TySucc hs ->
+       1 + (elab_exp hs ve)
+  | TyNRec h1 h2 h3 ->
+       let v1 = elab_exp h1 ve in
+       let v2 : elab_typ t = elab_exp h2 ve in
+       let v3 : elab_typ (TArr t t) = elab_exp h3 ve in
+       fnrec #(elab_typ t) v1 v2 v3
+  | TyInl #_ #_ #t1 #t2 h1 ->
+       let v = elab_exp h1 ve in
+       Inl #(elab_typ t1) #(elab_typ t2) v
+  | TyInr #_ #_ #t1 #t2 h1 ->
+       let v = elab_exp h1 ve in
+       Inr #(elab_typ t1) #(elab_typ t2) v
+  | TyCase #_ #_ #_ #_ #t1 #t2 #t3 h1 h2 h3 ->
+       let v1 = elab_exp h1 ve in
+       let v2 = elab_exp h2 ve in
+       let v3 = elab_exp h3 ve in
+       (match v1 with | Inl x -> v2 x | Inr y -> v3 y)
+  | TyVar x -> ve x
+  | TyLam t1 #_ #t2 h1 ->
+       assert (t == TArr t1 t2);
+       let w : elab_typ t1 -> Tot (elab_typ t2) =
+         (fun x -> elab_exp h1 (vextend x ve)) in
+       cast_TArr w
+  | TyApp #_ #_ #_ #t1 #t2 h1 h2 ->
+       assert ((elab_typ t) == (elab_typ t2));
+       (* TODO: Should we change the order here, first evaluate argument? *)
+       let v1 : elab_typ (TArr t1 t2) = elab_exp h1 ve in
+       let v2 : elab_typ t1 = elab_exp h2 ve in
+       v1 v2
+  | TyFst #_ #_ #t1 #t2 h1 ->
+       let v = elab_exp h1 ve in
+       fst #(elab_typ t1) #(elab_typ t2) v
+  | TySnd #_ #_ #t1 #t2 h1 ->
+       let v = elab_exp h1 ve in
+       snd #(elab_typ t1) #(elab_typ t2) v
+  | TyPair #_ #_ #_ #t1 #t2 h1 h2 ->
+       let v1 = elab_exp h1 ve in
+       let v2 = elab_exp h2 ve in
+       (v1, v2)
+//   | TyStringLit s -> s
+//   | TyByteLit b -> b
+//   | TyBytesCreate h1 h2 ->
+//        let v1 : elab_typ TNat = elab_exp h1 ve in
+//        let v2 : elab_typ TByte = elab_exp h2 ve in
+//        let b : bytes = Bytes.create (convert v1) v2 in
+//        b
+
+let thunk_exp #e #t (ht:typing empty e t) : e':exp & (typing empty e' (TArr TUnit t)) =
+     admit ();
+     (| ELam TUnit e, TyLam TUnit ht |)
+
+(** ** Properties of eval elab **)
+
+let rec eval_esucc_commute (#e:exp) (ht:typing empty e TNat)
+  : Lemma (ensures (
+    let ht : typing empty e TNat = ht in
+    let (| e', ht' |) = eval ht in
+    let (| e'', ht'' |) = eval (TySucc ht) in
+    ESucc e' == e'' /\
+    TySucc ht' == ht''
+  )) (decreases ht) =
+  if is_value e then ()
+  else begin
+    calc (==) {
+      eval #(ESucc e) (TySucc ht);
+      == {}
+      (let (| e', s |) = progress ht in
+      eval #(ESucc e') (TySucc (preservation_step ht s)));
+    };
+    let (| e', s |) = progress ht in
+    let ht' = preservation_step ht s in
+    assume (ht' << ht); (** TODO: proof of termination **)
+    eval_esucc_commute ht'
+  end
+
+let rec elab_invariant_to_eval #e #t (ht:typing empty e t)
+  : Lemma (elab_exp ht vempty == elab_exp (dsnd (eval ht)) vempty) =
+  match ht with
+  | TyUnit -> ()
+  | TyZero -> ()
+  | TySucc hts ->
+      calc (==) {
+        elab_exp (TySucc hts) vempty;
+        == { }
+        1 + elab_exp hts vempty;
+        == {  elab_invariant_to_eval hts }
+        1 + elab_exp (dsnd (eval hts)) vempty;
+        == { } 
+        elab_exp (TySucc (dsnd (eval hts))) vempty;
+        == { eval_esucc_commute hts }
+        elab_exp (dsnd (eval (TySucc hts))) vempty;
+      }
+  | _ -> admit ()
